refactoring: module names

ffi/console.ml
@@ -1,2 +1,2 @@
-let read_nat = read_int
+let read_int = read_int
 let write = print_endline
